theories/tree_borrows/defs.v
@@ -13,28 +13,41 @@ Definition wf_mem_tag (h: mem) (nxtp: tag) :=
   ∀ (l l':loc) pid, h !! l = Some (ScPtr l' pid) →
     (pid < nxtp)%nat.
 
-Definition wf_item_fresh (it:item) (nxtp:tag) (nxtc:call_id) :=
+Definition item_wf (it:item) (nxtp:tag) (nxtc:call_id) :=
   (forall tg, IsTag tg it -> (tg < nxtp)%nat)
   /\ (forall cid, protector_is_for_call cid (iprot it) -> (cid < nxtc)%nat).
 
-Definition wf_tree_fresh (tr:tree item) (nxtp:tag) (nxtc:call_id) :=
-  every_node (fun it => wf_item_fresh it nxtp nxtc) tr.
 
-Definition wf_trees_fresh (trs:trees) (nxtp:tag) (nxtc:call_id) :=
-  ∀ blk tr, trs !! blk = Some tr → wf_tree_fresh tr nxtp nxtc.
+Definition tree_items_unique (tr:tree item) :=
+  forall tg,
+  tree_contains tg tr -> exists it,
+    tree_unique tg tr
+    /\ tree_item_determined tg it tr.
 
-Definition wf_tree_nodup (tr:tree item) :=
-  forall tg, tree_contains tg tr -> tree_unique tg tr.
+Definition tree_items_compat_nexts (tr:tree item) (nxtp:tag) (nxtc: call_id) :=
+  every_node (λ it, item_wf it nxtp nxtc) tr.
+  (* FIXME: unique *)
 
-Definition wf_trees_nodup (trs:trees) :=
-  ∀ blk tr, trs !! blk = Some tr → wf_tree_nodup tr.
-
+(* FIXME: consistent naming *)
+Definition wf_tree (tr:tree item) :=
+  tree_items_unique tr.
+Definition each_tree_wf (trs:trees) :=
+  ∀ blk tr, trs !! blk = Some tr → wf_tree tr.
+Definition tags_unique_per_location (trs:trees) :=
+  ∀ blk1 blk2 tr1 tr2 tg, trs !! blk1 = Some tr1 → trs !! blk2 = Some tr2 →
+          tree_contains tg tr1 → tree_contains tg tr2 → blk1 = blk2.
+Definition wf_trees (trs:trees) :=
+  each_tree_wf trs ∧ tags_unique_per_location trs.
+Definition trees_compat_nexts (trs:trees) (nxtp:tag) (nxtc: call_id) :=
+  ∀ blk tr, trs !! blk = Some tr → tree_items_compat_nexts tr nxtp nxtc.
 Definition wf_non_empty (trs:trees) :=
   ∀ blk tr, trs !! blk = Some tr → tr ≠ empty.
-
+(*
+Definition wf_no_dup (α: stacks) :=
+  ∀ l stk, α !! l = Some stk → NoDup stk.
+*)
 Definition wf_cid_incl (cids: call_id_set) (nxtc: call_id) :=
   ∀ c : call_id, c ∈ cids → (c < nxtc)%nat.
-
 Definition wf_scalar t sc := ∀ t' l, sc = ScPtr l t' → t' < t.
 
 (* mem ~ gmap loc scalar
@@ -51,8 +64,8 @@ Record state_wf (s: state) := {
   (*state_wf_dom : dom s.(shp) ≡ dom s.(strs); Do we care ? After all TB is very permissive about the range, so out-of-bounds UB is *always* triggered at the level of the heap, not the trees *)
   state_wf_dom : same_blocks s.(shp) s.(strs);
   (*state_wf_mem_tag : wf_mem_tag s.(shp) s.(snp);*) (* FIXME: this seems to state that all pointers are wf, it should be included *)
-  state_wf_tree_fresh : wf_trees_fresh s.(strs) s.(snp) s.(snc);
-  state_wf_tree_nodup : wf_trees_nodup s.(strs);
+  state_wf_tree_unq : wf_trees s.(strs);
+  state_wf_tree_compat : trees_compat_nexts s.(strs) s.(snp) s.(snc);
   state_wf_non_empty : wf_non_empty s.(strs);
   (*state_wf_cid_no_dup : NoDup s.(scs) ;*) (* FIXME: call ids are unique, include this *)
   state_wf_cid_agree: wf_cid_incl s.(scs) s.(snc);
